{\bf 07.02}
\begin{equation*}
\begin{gathered}
	F(x)=\bigg\{ -\frac{1}{x^{2}}, \text{all real x} \\
\end{gathered}
\end{equation*}


2a. $F_{X_{n:n}}(y)= (\frac{1}{1+e^{-y}})^{n} ; \lim _{n\to \infty } 
(\frac{1}{1+e^{-y}})^{n}$ has no limiting distribution. \\

2b. $F_{X_{n:n}-\ln (n)}(y)= P\lbrack X_{n:n}-\ln (n)\le y\rbrack = 
P\lbrack X_{n:n}\le y+\ln (n)\rbrack $\\


$= F_{X_{n:n}} (y+\ln (n))^{n}= (\frac{1}{1+e^{-(y+\ln (n))}})^{n}= 
(\frac{1}{1+\frac{e^{-y}}{n}})^{n};$\\


$\lim _{n\to \infty } (\frac{1}{1+\frac{e^{-y}}{n}})^{n}= e^{-e^{-y}}$
\\
