
{\bf 07.03}
\textbf{3a.}
$F(x)=\bigg\{ 
\begin{gathered}
1-\frac{1}{x^{2}}, x>1 \\
0, x\le 0 \\
\end{gathered}
$\\




$F_{X_{1:n}}(y)= P\lbrack X_{1:n} \le y\rbrack = 1- P\lbrack X_{1:n} 
\ge y\rbrack =1-\frac{1}{y^{2n}} , y>1$\\


$\lim _{n\to \infty }(1-\frac{1}{y^{2n}})=1-0= \bigg\{ 
\begin{gathered}
1, y>1 \\
0, y\le 0 \\
\end{gathered}
$\\




\textbf{3b.}



$F_{X_{n:n}}(y)= P\lbrack X_{n:n} \le y\rbrack =1-P\lbrack X_{n:n} \ge 
y\rbrack = 1-(1-\frac{1}{y^{2}})^{n}= \frac{1}{y^{2n }} ;$ $lim?_{n\to 
\infty } \frac{1}{y^{2n }}$ = 0,

Therefore $F_{X_{n:n}}(y)$ has no limiting distribution.



\textbf{3c.}

$F_{n^{-\frac{1}{2 }}X_{n:n}}(y)= P\lbrack \frac{1}{\sqrt{n}}X_{n:n} 
\le y\rbrack = P\lbrack X_{n:n} \le \sqrt{n}y\rbrack 
=F_{X_{n:n}}(\sqrt{n}y) =(1- (\sqrt{n}y)^{-2})^{n}, for 
y>\frac{1}{\sqrt{n}}$\\


$\lim _{n\to \infty }(1- (\sqrt{n}y)^{-2})^{n}= 
(1-\frac{1}{ny^{2}})^{n}=\bigg\{ 
\begin{gathered}
 e^{-y^{-2}}, y>0 \\
0, y\le 0 \\
\end{gathered}
 $\\