{\bf 08.04} \\
 
Using a change of variables: \quad $X_1 = \frac{Y_1 + Y_2}{2}, \quad X_2 = \frac{Y_1 - Y_2}{2}$ \\
 
J = det = $ - \frac{1}{2}$ \\
 
$f_y{(y_1,y_2)} = f_x{\left (\frac{Y_1 + Y_2}{2},\frac{Y_1 - Y_2}{2} \right)}$ \\
 
$ = \frac{1}{2 \pi \sigma^2}exp{\frac{1}{2 \sigma^2}}\Big[{\left (\frac{Y_1 + Y_2}{2} \right)^2 + \left (\frac{Y_1 - Y_2}{2} \right)^2}\Big]$ \\
 
$ = \frac{1}{2 \pi \sigma^2}exp{\frac{1}{2 \sigma^2}}{\left (\frac{Y_1^2}{4} + \frac{Y_2^2}{4} + \frac{Y_1^2}{4} + \frac{Y_2^2}{4} \right)}$ \\
 
$ = \frac{1}{2 \pi \sigma^2}exp{\frac{1}{2 \sigma^2}}{\left (\frac{Y_1^2}{4} + \frac{Y_1^2}{4} \right) + \left (\frac{Y_2^2}{4} + \frac{Y_2^2}{4} \right)}$ \\
 
$ = \frac{1}{2 \pi \sigma^2}exp{\frac{1}{2 \sigma^2}}\Big[{\left (\frac{Y_1}{2} \right)^2 + \left (\frac{Y_2}{2} \right)^2}\Big]$ \\
 
Hence, $f_y{(y_1,y_2)} = f_x{\left (\frac{Y_1 + Y_2}{2},\frac{Y_1 - Y_2}{2} \right)}$ = $f_{x1}{(Y_1)},f_{x2}{(Y_2)}$ \\
 
Therefore $Y_1$ and $Y_2$ are independent and normally distributed. \\
